\documentclass{article}

\usepackage{amssymb}
\usepackage{amsmath}

\begin{document}

\title{Problem Set 1}
\maketitle


\noindent 3. Prove or disprove the following about regular expressions r, s, t where r=s implies L(r)=L(s)

\noindent     (d) (r+s)* = r* + s*

\noindent 

Let $\boldsymbol{\mathrm{\Sigma }}\boldsymbol{=}\left\{\boldsymbol{0},\boldsymbol{1}\right\}$

Let \textbf{r = 0*} and \textbf{s = 1*}

 Then, ${\left(r+s\right)}^*=\epsilon \cup \left\{1,0\right\}\cup {\left\{1,0\right\}}^2\cup {\left\{1,0\right\}}^3\cup \dots $

 And, $r^*+s^*=\epsilon \cup \left\{1\right\}\cup {\left\{1\right\}}^2\cup {\left\{1\right\}}^3\cup \dots \cup \left\{0\right\}\cup {\left\{0\right\}}^2\cup {\left\{0\right\}}^3\cup \dots $

Now, consider a string $\boldsymbol{01}$

$\boldsymbol{01}\in {\left\{1,0\right\}}^2\ \ \Rightarrow \ \ \ \ \boldsymbol{01}\in {\left(r+s\right)}^*$

 But clearly,    $01\notin r^*+s^*$

Hence, (r+s)* $\neq $ r* + s*

\noindent 


\end{document}

